src/program_proof/chat/merkle/merkle.v
@@ -15,7 +15,7 @@ Context `{!heapGS Σ}.
 Definition own ptr arg : iProp Σ :=
   ∃ sl_B,
   "HB" ∷ own_slice_small sl_B byteT 1 arg.(B) ∗
-  "HB_ptr" ∷ ptr ↦[Id :: "B"] (slice_val sl_B).
+  "Hptr_B" ∷ ptr ↦[Id :: "B"] (slice_val sl_B).
 End local_defs.
 End Id.
 
@@ -30,23 +30,26 @@ Context `{!heapGS Σ}.
 Definition own ptr arg : iProp Σ :=
   ∃ sl_B,
   "HB" ∷ own_slice_small sl_B byteT 1 arg.(B) ∗
-  "HB_ptr" ∷ ptr ↦[Id :: "B"] (slice_val sl_B).
+  "Hptr_B" ∷ ptr ↦[Id :: "B"] (slice_val sl_B).
 End local_defs.
+
+Definition encodesF (arg:t) : list u8 :=
+  arg.(B).
 End Val.
 
-Section proof.
+Section tree.
 Context `{!heapGS Σ}.
 
 (* TODO: will need to carry some invariant that the # of children == 256. *)
 Inductive tree : Type :=
   | Leaf : list u8 → tree
-  | ChildNode : list (option tree) → tree.
+  | Interior : list (option tree) → tree.
 
 Definition tree_to_map (t : tree) : gmap (list u8) (list u8) :=
   let fix traverse (t : tree) (acc : gmap (list u8) (list u8)) (path : list u8) :=
     match t with
     | Leaf val => <[path:=val]>acc
-    | ChildNode children =>
+    | Interior children =>
       (* Grab all entries from the children, storing the ongoing path. *)
       (foldr
         (λ child (p:(Z * gmap (list u8) (list u8))),
@@ -67,7 +70,7 @@ Definition is_tree_hash' (recur : tree -d> list u8 -d> iPropO Σ) : tree -d> lis
   (λ t h,
   match t with
   | Leaf val => is_hash val h
-  | ChildNode children =>
+  | Interior children =>
       ∃ (child_hashes : list (list u8)),
       ([∗ list] child;hash ∈ children;child_hashes,
         match child with
@@ -82,6 +85,146 @@ Proof. solve_contractive. Qed.
 
 Definition is_tree_hash : tree → list u8 → iProp Σ := fixpoint is_tree_hash'.
 
+Definition own_tree' (recur : loc -d> tree -d> iPropO Σ) : loc -d> tree -d> iPropO Σ :=
+  (λ ptr arg,
+    match arg with
+    | Leaf val =>
+      ∃ ptr_v v hash sl_hash sl_children,
+      "Hval" ∷ Val.own ptr_v v ∗
+      "Hptr_val" ∷ ptr ↦[Node :: "Val"] #ptr_v ∗
+      "#His_hash" ∷ is_tree_hash arg hash ∗
+      "Hhash" ∷ own_slice_small sl_hash byteT 1 hash ∗
+      "Hsl_hash" ∷ ptr ↦[Node :: "hash"] (slice_val sl_hash) ∗
+      "Hchildren" ∷ own_slice_small sl_children ptrT 1 (replicate 256 null) ∗
+      "Hsl_children" ∷ ptr ↦[Node :: "Children"] (slice_val sl_children)
+    | Interior children =>
+      ∃ hash sl_hash sl_children ptr_children,
+      "Hptr_val" ∷ ptr ↦[Node :: "Val"] #null ∗
+      "#His_hash" ∷ is_tree_hash arg hash ∗
+      "Hhash" ∷ own_slice_small sl_hash byteT 1 hash ∗
+      "Hsl_children" ∷ own_slice_small sl_children ptrT 1 ptr_children ∗
+      "Hptr_children" ∷ ptr ↦[Node :: "Children"] (slice_val sl_children) ∗
+      "Hchildren" ∷
+        ([∗ list] child;ptr_child ∈ children;ptr_children,
+          match child with
+          | None => ⌜ptr_child = null⌝
+          | Some t' => ▷ recur ptr_child t'
+          end)
+    end)%I.
 
+Local Instance own_tree'_contractive : Contractive own_tree'.
+Proof. solve_contractive. Qed.
+
+Definition own_tree : loc → tree → iProp Σ := fixpoint own_tree'.
+
+Lemma own_tree_unfold ptr arg :
+  own_tree ptr arg ⊣⊢
+  match arg with
+  | Leaf val =>
+    ∃ ptr_v v hash sl_hash sl_children,
+    "Hval" ∷ Val.own ptr_v v ∗
+    "Hptr_val" ∷ ptr ↦[Node :: "Val"] #ptr_v ∗
+    "#His_hash" ∷ is_tree_hash arg hash ∗
+    "Hhash" ∷ own_slice_small sl_hash byteT 1 hash ∗
+    "Hsl_hash" ∷ ptr ↦[Node :: "hash"] (slice_val sl_hash) ∗
+    "Hchildren" ∷ own_slice_small sl_children ptrT 1 (replicate 256 null) ∗
+    "Hsl_children" ∷ ptr ↦[Node :: "Children"] (slice_val sl_children)
+  | Interior children =>
+    ∃ hash sl_hash sl_children ptr_children,
+    "Hptr_val" ∷ ptr ↦[Node :: "Val"] #null ∗
+    "#His_hash" ∷ is_tree_hash arg hash ∗
+    "Hhash" ∷ own_slice_small sl_hash byteT 1 hash ∗
+    "Hsl_children" ∷ own_slice_small sl_children ptrT 1 ptr_children ∗
+    "Hptr_children" ∷ ptr ↦[Node :: "Children"] (slice_val sl_children) ∗
+    "Hchildren" ∷
+      ([∗ list] child;ptr_child ∈ children;ptr_children,
+        match child with
+        | None => ⌜ptr_child = null⌝
+        | Some t' => ▷ own_tree ptr_child t'
+        end)
+  end.
+Proof. apply (fixpoint_unfold own_tree'). Qed.
+End tree.
+
+Module RootedTree.
+Record t :=
+  mk {
+    Root: tree;
+    PtrRoot: loc;
+  }.
+
+Section local_defs.
+Context `{!heapGS Σ}.
+Definition own ptr arg : iProp Σ :=
+  "Hroot" ∷ own_tree arg.(PtrRoot) arg.(Root) ∗
+  "Hptr_root" ∷ ptr ↦[Tree :: "Root"] #arg.(PtrRoot).
+End local_defs.
+End RootedTree.
+
+Section proof.
+Context `{!heapGS Σ}.
+
+Lemma wp_InteriorHash children ptr_tree old_hash sl_children ptr_children :
+  {{{
+    "Hptr_val" ∷ ptr_tree ↦[Node :: "Val"] #null ∗
+    "Hhash" ∷ ptr_tree ↦[Node :: "hash"] old_hash ∗
+    "Hsl_children" ∷ own_slice_small sl_children ptrT 1 ptr_children ∗
+    "Hstruct_children" ∷ ptr_tree ↦[Node :: "Children"] sl_children ∗
+    "Hchildren" ∷
+      ([∗ list] child;ptr_child ∈ children;ptr_children,
+        match child with
+        | None => ⌜ptr_child = null⌝
+        | Some t' => ▷ own_tree ptr_child t'
+        end)
+  }}}
+  Node__UpdateInteriorHash #ptr_tree
+  {{{
+    RET #();
+    own_tree ptr_tree (Interior children)
+  }}}.
+Proof. Admitted.
+
+Lemma sep_nil_children :
+ ⊢
+ ([∗ list] child;ptr_child ∈ replicate 256 None;replicate (int.nat 256) null,
+   match child with
+   | Some t' => ▷ own_tree ptr_child t'
+   | None => ⌜ptr_child = null⌝
+   end).
+Proof.
+  replace (int.nat 256) with (256%nat); [|word].
+  naive_solver.
+Qed.
+
+Lemma wp_NewTree :
+  {{{ True }}}
+  NewTree #()
+  {{{
+    ptr_tree ptr_root, RET #ptr_tree;
+    RootedTree.own ptr_tree (RootedTree.mk (Interior (replicate 256 None)) ptr_root)
+  }}}.
+Proof.
+  iIntros (Φ) "_ HΦ".
+  rewrite /NewTree.
+  wp_apply wp_allocStruct; [val_ty|].
+  iIntros (ptr_node) "H".
+  iDestruct (struct_fields_split with "H") as "H"; iNamed "H".
+  wp_apply wp_NewSlice.
+  iIntros (sl_children) "H".
+  iDestruct (own_slice_to_small with "H") as "Hsl_children".
+  wp_apply (wp_storeField with "[$]"); [val_ty|].
+  iIntros "Hchildren".
+  wp_apply (wp_InteriorHash with "[$Val $hash $Hsl_children $Hchildren]").
+  {
+    instantiate (1:=(replicate 256 None)).
+    iApply sep_nil_children.
+  }
+  iIntros "Htree".
+  wp_apply wp_allocStruct; [val_ty|].
+  iIntros (ptr_tree) "H".
+  iDestruct (struct_fields_split with "H") as "H"; iNamed "H".
+  iApply "HΦ".
+  iFrame.
+Qed.
 
 End proof.
